Extraction.lean
@@ -8,10 +8,34 @@ inductive P : Nat → Nat → Nat → Prop
 inductive Q : Prop
   | intro
 
-@[grind =]
-theorem p_iff_q : P 1 2 3 ↔ Q := by
+section NoFVars
+
+theorem p_eq_q : P 1 2 3 = Q := by
   simp [P.intro, Q.intro]
 
+theorem p_heq_q : P 1 2 3 ≍ Q := by
+  simp [P.intro, Q.intro]
+
+/--
+error: unsolved goals
+⊢ Q
+-/
+#guard_msgs in
 example : P 1 2 3 := by
+  grind [p_eq_q] extract min_ast
+
+/--
+error: unsolved goals
+⊢ Q
+-/
+#guard_msgs in
+example : P 1 2 3 := by
+  grind [p_heq_q] extract min_ast
+
+end NoFVars
+
+/-- error: (kernel) declaration has free variables '_example' -/
+#guard_msgs in
+example (h : P 1 2 3 ↔ Q) : P 1 2 3 := by
   grind extract min_ast
   constructor
