Extraction/Lean.lean
@@ -1,0 +1,11 @@
+import Lean
+
+def HEq.mp {α β : Sort u} (h : α ≍ β) (a : α) : β :=
+  eq_of_heq h ▸ a
+
+def Lean.Meta.mkHEqMP (heqProof pr : Expr) : MetaM Expr :=
+  mkAppM ``HEq.mp #[heqProof, pr]
+
+def Lean.Meta.mkEqHEqMP (eqHEqProof pr : Expr) : MetaM Expr := do
+  let type ← inferType eqHEqProof
+  if type.isEq then mkEqMP eqHEqProof pr else mkHEqMP eqHEqProof pr
